src/cbor/pulse/raw/everparse/CBOR.Pulse.Raw.EverParse.Det.Compare.Dispatch.String.fsti
@@ -1,0 +1,32 @@
+module CBOR.Pulse.Raw.EverParse.Det.Compare.Dispatch.String
+#lang-pulse
+include CBOR.Pulse.Raw.EverParse.Det.Compare.Base
+open CBOR.Spec.Raw.EverParse
+open CBOR.Pulse.Raw.EverParse.Type
+open CBOR.Pulse.Raw.EverParse.Match
+open CBOR.Pulse.Raw.EverParse.Match.Fuel
+open CBOR.Pulse.Raw.EverParse.Access
+open CBOR.Pulse.Raw.Compare.Base
+open CBOR.Pulse.Raw.Compare.Bytes
+open Pulse.Lib.Pervasives
+open Pulse.Lib.Trade
+
+module I16 = FStar.Int16
+module Trade = Pulse.Lib.Trade.Util
+
+inline_for_extraction
+val cbor_compare_dispatch_string_case
+  (n: Ghost.erased nat { Ghost.reveal n >= 1 })
+  (x1: cbor_raw)
+  (x2: cbor_raw)
+  (#pm1: perm) (#v1: Ghost.erased raw_data_item)
+  (#pm2: perm) (#v2: Ghost.erased raw_data_item)
+: stt I16.t
+    (cbor_raw_match_fuel n pm1 x1 v1 **
+     cbor_raw_match_fuel n pm2 x2 v2 **
+     pure (String? (Ghost.reveal v1) /\ String? (Ghost.reveal v2) /\
+           String?.typ (Ghost.reveal v1) == String?.typ (Ghost.reveal v2)))
+    (fun res ->
+      cbor_raw_match_fuel n pm1 x1 v1 **
+      cbor_raw_match_fuel n pm2 x2 v2 **
+      pure (same_sign (I16.v res) (cbor_compare v1 v2)))
